SEARordinal.sml
@@ -1,0 +1,544 @@
+(*ordinal with base set as a quotient of well orders*)
+
+val Holdm_def = qdefine_psym("Holdm",[‘r:mem(Pow(A * B))’,‘a:mem(A)’,‘b:mem(B)’]) ‘IN(Pair(a,b),r)’
+                            |> gen_all
+
+val rdom_def = 
+    IN_def_P |> spec_all 
+             |> fVar_sInst_th “P(a:mem(A))”
+                “?a1:mem(A). Holdm(r,a:mem(A),a1)”
+             |> uex2ex_rule |> qSKOLEM "rdom" [‘r’] 
+             |> gen_all
+
+val rcod_def = 
+    IN_def_P |> spec_all 
+             |> fVar_sInst_th “P(a:mem(A))”
+                “?a1:mem(A). Holdm(r,a1,a:mem(A))”
+             |> uex2ex_rule |> qSKOLEM "rcod" [‘r’] 
+             |> gen_all
+
+val rset_def = qdefine_fsym("rset",[‘r:mem(Pow(A*A))’])
+‘Union(rdom(r),rcod(r))’ |> gen_all
+
+val strict_def =
+    IN_def_P |> qspecl [‘A * A’] 
+             |> fVar_sInst_th “P(a12:mem(A*A))”
+             “Holdm(r:mem(Pow(A*A)),Fst(a12),Snd(a12)) & 
+             ~(Fst(a12) = Snd(a12))”
+        |> uex2ex_rule |> qSKOLEM "strict" [‘r’]
+        |> qspecl [‘Pair(a1:mem(A),a2:mem(A))’]
+        |> rewr_rule[Pair_def']
+        |> gen_all
+
+val wellfounded_def = qdefine_psym("wellfounded",
+[‘r:mem(Pow(A*A))’])
+‘!s. (?w. IN(w,s)) ==> ?min.IN(min,s) & 
+     !w. Holdm(r,w,min) ==> ~IN(w,s)’
+     |> gen_all
+
+val reflexive_def = qdefine_psym("reflexive",
+[‘r:mem(Pow(A * A))’,‘s:mem(Pow(A))’])
+‘!x. IN(x,s) ==> Holdm(r,x,x)’ |> gen_all
+
+val transitive_def = qdefine_psym("transitive",
+[‘r:mem(Pow(A*A))’])
+‘!x y z. Holdm(r,x,y) & Holdm(r,y,z) ==> Holdm(r,x,z)’
+|> gen_all
+
+val antisym_def = qdefine_psym("antisym",
+[‘r:mem(Pow(A*A))’])
+‘!x y.Holdm(r,x,y) & Holdm(r,y,x) ==> x = y’
+
+val linear_order_def = qdefine_psym("linear_order",
+[‘r:mem(Pow(A*A))’,‘s:mem(Pow(A))’])
+‘SS(rdom(r),s) & SS(rcod(r),s) &
+ transitive(r) & antisym(r) &
+ (!x y. IN(x,s) & IN(y,s) ==> Holdm(r,x,y) | Holdm(r,y,x))’
+|> gen_all
+
+val wellorder_def = qdefine_psym("wellorder",[‘r:mem(Pow(A*A))’])
+‘wellfounded(strict(r)) &
+ linear_order(r,rset(r)) &
+ reflexive(r,rset(r))’|> gen_all
+
+
+val WO_def = Thm_2_4 |> qspecl [‘Pow(A*A)’] 
+                     |> fVar_sInst_th “P(r:mem(Pow(A*A)))”
+                     “wellorder(r:mem(Pow(A*A)))”
+                     |> qSKOLEM "WO" [‘A’] 
+                     |> qSKOLEM "iWO" [‘A’] 
+                     |> gen_all 
+
+
+val Rwo_def = qdefine_fsym("Rwo",[‘wo:mem(WO(A))’])
+‘App(iWO(A),wo)’ |> gen_all
+
+val WIN_def = qdefine_psym("WIN",[‘w:mem(WO(A))’,‘x:mem(A)’,
+‘y:mem(A)’]) ‘Holdm(strict(Rwo(w)),x,y)’ |> gen_all
+
+val iseg_def = IN_def_P |> spec_all 
+                        |> fVar_sInst_th “P(y:mem(A))”
+                           “WIN(w:mem(WO(A)),y,x)”
+                        |> uex2ex_rule
+                        |> qSKOLEM "iseg" [‘w’,‘x’]
+                        |> gen_all
+
+(*
+val lt_def = qdefine_psym("lt",[‘r:mem(Pow(A*A))’,
+                                  ‘a1:mem(A)’,‘a2:mem(A)’])
+‘Holdm(r,a1,a2) & ~(a1 = a2)’ |> gen_all
+*)
+
+val elsOf_def = qdefine_fsym("elsOf",[‘w:mem(WO(A))’])
+‘rset(Rwo(w))’ |> gen_all
+
+val NOT_Holdm_Empty = prove_store("NOT_Holdm_Empty",
+e0
+(rw[Holdm_def,Empty_def])
+(form_goal “!A x y.~Holdm(Empty(A*A),x,y)”));
+
+val rdom_rcod_Empty = prove_store("rdom_rcod_Empty",
+e0
+(rw[rdom_def,rcod_def,GSYM IN_EXT_iff,
+    Empty_def,NOT_Holdm_Empty] >>
+ rpt strip_tac >> ccontra_tac >> fs[] )
+(form_goal “!A.rdom(Empty(A*A)) = Empty(A) &
+ rcod(Empty(A*A)) = Empty(A)”));
+
+val rset_Empty = prove_store("rset_Empty",
+e0
+(rw[rset_def,IN_Union,rdom_rcod_Empty,Empty_def,
+    Union_Empty_Empty])
+(form_goal “!A.rset(Empty(A*A)) = Empty(A)”));
+
+val strict_Empty_Empty= prove_store("strict_Empty_Empty",
+e0
+(rw[GSYM IN_EXT_iff] >>
+ fconv_tac (redepth_fconv no_conv forall_cross_fconv) >>
+ rw[strict_def,Empty_def,NOT_Holdm_Empty])
+(form_goal “!A. strict(Empty(A*A)) = Empty(A*A)”));
+
+val Empty_wellfounded = prove_store("Empty_wellfounded",
+e0
+(rw[wellfounded_def,Empty_def,NOT_Holdm_Empty])
+(form_goal
+ “!A. wellfounded(Empty(A*A))”));
+
+val Empty_reflexive = prove_store("Empty_reflexive",
+e0
+(rw[reflexive_def,Empty_def])
+(form_goal “!A. reflexive(Empty(A * A),Empty(A))”));
+
+
+val Empty_transitive = prove_store("Empty_transitive",
+e0
+(rw[transitive_def,Empty_def,NOT_Holdm_Empty])
+(form_goal “!A. transitive(Empty(A * A))”));
+
+
+val Empty_antisym = prove_store("Empty_antisym",
+e0
+(rw[antisym_def,Empty_def,NOT_Holdm_Empty])
+(form_goal “!A. antisym(Empty(A * A))”));
+
+val Empty_linear_order = prove_store("Empty_linear_order",
+e0
+(rw[linear_order_def,rdom_rcod_Empty,SS_Refl,Empty_def,
+    Empty_antisym,Empty_transitive])
+(form_goal “!A.linear_order(Empty(A * A), Empty(A))”));
+
+
+val Empty_wellorder = prove_store("Empty_wellorder",
+e0
+(strip_tac >> rw[wellorder_def,strict_Empty_Empty,
+                 Empty_wellfounded,Empty_reflexive,
+                 rset_Empty,Empty_linear_order])
+(form_goal “!A.wellorder(Empty(A*A))”));
+
+val WO_uex = prove_store("WO_uex",
+e0
+(rpt strip_tac >> rw[Rwo_def] >> 
+ irule $ iffRL Inj_ex_uex >> flip_tac >>
+ rw[GSYM WO_def] >> arw[])
+(form_goal
+ “!A r:mem(Pow(A*A)). wellorder(r) ==>
+      ?!w. Rwo(w) = r”));
+
+val zwo_def = WO_uex |> qsspecl [‘Empty(A*A)’]
+                     |> rewr_rule[Empty_wellorder]
+                     |> uex2ex_rule |> qSKOLEM "zwo" [‘A’]
+                     |> gen_all
+
+val Abswo_def = qdefine_fsym("Abswo",[‘A’])
+‘LINV(iWO(A),zwo(A))’ |> gen_all 
+
+val mkWO = qdefine_fsym("mkWO",[‘r:mem(Pow(A*A))’])
+‘App(Abswo(A),r)’ |> gen_all
+
+val orderiso_def = qdefine_psym("orderiso",[‘r1:mem(WO(A))’,
+                                      ‘r2:mem(WO(B))’])
+‘?f:A->B.
+ (!x. IN(x,elsOf(r1)) ==> IN(App(f,x),elsOf(r2))) &
+ (!x1 x2.IN(x1,elsOf(r1)) & IN(x2,elsOf(r1)) ==>
+  (App(f,x1) = App(f,x2) <=> x1 = x2)) & 
+ (!y. IN(y,elsOf(r2)) ==> ?x. IN(x,elsOf(r1)) & App(f,x) = y) &
+ (!x y. WIN(r1,x,y) ==> WIN(r2,App(f,x),App(f,y)))’
+|> gen_all
+
+val oiso_def = 
+AX1 |> qspecl [‘WO(A)’,‘WO(A)’] 
+    |> fVar_sInst_th “P(r1:mem(WO(A)),r2:mem(WO(A)))”
+       “orderiso(r1:mem(WO(A)),r2:mem(WO(A)))”
+    |> uex2ex_rule |> qSKOLEM "oiso" [‘A’] 
+    |> qspecl [‘r1:mem(WO(A))’,‘r2:mem(WO(A))’]
+    |> gen_all
+
+
+
+val rrestrict_def = 
+    IN_def_P |> qspecl [‘A*A’] 
+             |> fVar_sInst_th “P(a12:mem(A * A))”
+                “Holdm(r,Fst(a12),Snd(a12)) &
+                 IN(Fst(a12),s:mem(Pow(A))) &
+                 IN(Snd(a12),s:mem(Pow(A)))”
+             |> uex2ex_rule
+             |> qSKOLEM "rrestrict" [‘r’,‘s’]
+             |> qspecl [‘Pair(a1:mem(A),a2:mem(A))’] 
+             |> gen_all
+
+val wobound_def = qdefine_fsym("wobound",[‘x:mem(A)’,‘w:mem(WO(A))’]) ‘mkWO(rrestrict(Rwo(w),iseg(w,x)))’
+|> gen_all
+
+val WIN_wobound = prove_store("WIN_wobound",
+e0
+(cheat)
+(form_goal “!A x:mem(A) y z w.WIN(wobound(z,w),x,y) <=> 
+ WIN(w,x,z) & WIN(w,y,z) & WIN(w,x,y) ”));
+
+val wobound2 = prove_store("wobound2",
+e0
+(cheat)
+(form_goal “!A w a:mem(A) b.WIN(w,a,b) ==>
+ wobound(a,wobound(b,w)) = wobound(a,w)”));
+
+val orderlt_def = qdefine_psym("orderlt",
+[‘w1:mem(WO(A))’,‘w2:mem(WO(B))’])
+‘?x. IN(x,elsOf(w2)) & orderiso(w1,wobound(x,w2))’
+|> gen_all
+
+val orderlt_trichotomy = prove_store("orderlt_trichotomy",
+e0
+(cheat)
+(form_goal “!A B w1:mem(WO(A)) w2:mem(WO(B)).orderlt(w1,w2) | orderiso(w1,w2) | orderlt(w2,w1)”));
+
+val ordinal_def = 
+    Thm_2_4 |> qspecl [‘Pow(WO(A))’] 
+            |> fVar_sInst_th “P(a:mem(Pow(WO(A))))”
+               “?w.a = rsi(oiso(A),w)”
+            |> qSKOLEM "ordinal" [‘A’] 
+            |> qSKOLEM "iord" [‘A’] 
+
+
+
+val ordinal_uex = prove_store("ordinal_rsi_uex",
+e0
+(rpt strip_tac >> rw[Rwo_def] >> 
+ irule $ iffRL Inj_ex_uex >> flip_tac >>
+ rw[GSYM WO_def] >> arw[])
+(form_goal
+ “!A r:mem(Pow(A*A)). wellorder(r) ==>
+      ?!w. Rwo(w) = r”));
+
+
+val r2f_def = proved_th $
+e0
+cheat
+(form_goal “!R:A~>B. ?!f:A * B -> 1+1.
+ !a b. App(f,Pair(a,b)) = App(i2(1,1),dot)  <=> Holds(R,a,b)”)
+|> spec_all |> uex2ex_rule |> qSKOLEM "r2f" [‘R’] |> gen_all
+
+
+val oiso_ER = prove_store("oiso_ER",
+e0
+(cheat)
+(form_goal “!A. ER(oiso(A))”));
+
+val prrel_oiso_ER = prove_store("prrel_oiso_ER",
+e0
+(cheat)
+(form_goal “!A B. ER(prrel(oiso(A),oiso(B)))”));
+
+val oiso_iord_Quot = prove_store("oiso_iord_Quot",
+e0
+(cheat)
+(form_goal “Quot(oiso(A),iord(A))”));
+
+
+
+val oiso_iord_Quot_cong = prove_store("oiso_iord_Quot_cong",
+e0
+(cheat)
+(form_goal “!A.Quot(prrel(oiso(A),oiso(A)),
+                 ipow2(iord(A),iord(A)))”));
+
+val orderltr_def = 
+AX1 |> qspecl [‘WO(A)’,‘WO(A)’] 
+    |> fVar_sInst_th “P(w1:mem(WO(A)),w2:mem(WO(A)))”
+       “orderlt(w1:mem(WO(A)),w2:mem(WO(A)))”
+    |> uex2ex_rule |> qSKOLEM "orderltr" [‘A’] 
+    |> gen_all
+
+val resp1_r2f_orderltr = prove_store("resp1_r2f_orderltr",
+e0
+(cheat)
+(form_goal 
+ “!A.resp1(r2f(orderltr(A)), prrel(oiso(A), oiso(A))) ”));
+
+
+val zord_def = 
+  Quot_rsi_uex |> qsspecl [‘oiso(A)’,‘iord(A)’]
+               |> rewr_rule[oiso_iord_Quot] 
+               |> qspecl [‘zwo(A)’] 
+               |> uex2ex_rule 
+               |> qSKOLEM "zord" [‘A’]
+               |> gen_all
+
+val oiso_iord_abs_cong = 
+abs_cong |> qsspecl [‘oiso(A)’,‘iord(A)’,‘oiso(A)’,‘iord(A)’]
+         |> rewr_rule[oiso_ER,oiso_iord_Quot]
+
+val Abso_def = qdefine_fsym("Abso",[‘w:mem(WO(A))’])
+‘abs(oiso(A), iord(A), zord(A), w)’ |> gen_all
+
+val ordltf_def = 
+Quot_UMP |> qsspecl [‘prrel(oiso(A),oiso(A))’]
+         |> rewr_rule[prrel_oiso_ER]
+         |> qsspecl [‘r2f(orderltr(A))’]
+         |> rewr_rule[resp1_r2f_orderltr] 
+         |> qsspecl [‘ipow2(iord(A),iord(A))’] 
+         |> rewr_rule[oiso_iord_Quot_cong] 
+         |> qspecl [‘Pair(zord(A),zord(A))’]
+         |> uex2ex_rule
+         |> qSKOLEM "ordltf" [‘A’] 
+         |> qspecl [‘Pair(w1:mem(WO(A)),w2:mem(WO(A)))’] 
+         |> rewr_rule[oiso_iord_abs_cong,
+                      GSYM Abso_def]
+
+val ordlt_def = 
+qdefine_psym("ordlt",[‘ord1:mem(ordinal(A))’,‘ord2:mem(ordinal(A))’]) ‘App(ordltf(A), Pair(ord1, ord2)) = true’
+|> gen_all
+
+val ordltr_def = 
+AX1 |> qspecl [‘ordinal(A)’,‘ordinal(A)’] 
+    |> uex2ex_rule |> qSKOLEM "ordltr" [‘A’] 
+    |> qspecl [‘ord1:mem(ordinal(A))’,‘ord2:mem(ordinal(A))’] 
+    |> gen_all
+
+val ordltm_def = qdefine_fsym("ordltm",[‘A’])
+‘r2m(ordltr(A))’ |> gen_all
+
+val ordltm_wellorder = prove_store("ordltm_wellorder",
+e0
+cheat
+(form_goal “!A. wellorder(ordltm(A))”));
+
+
+(*
+Definition 4. Well-foundedness also allows the definition of a “least” operator for or-
+dinals:
+(oleast) (P : α ordinal → bool) =
+ε(x : αordinal).P x ∧ ∀(y : αordinal).y <x ⇒ ¬P y
+This is well-defined as long as the predicate (or set) P is not everywhere false (the empty set).
+*)
+
+
+val oleast_ex0 = proved_th $
+e0
+(rpt strip_tac >>
+ cheat)
+(form_goal 
+ “!A s:mem(Pow(ordinal(A))). (?ord. IN(ord,s)) ==> 
+        ?!x. IN(x,s) & !y. ordlt(y,x) ==> ~IN(y,s)”)
+
+val oleastf_ex = proved_th $
+e0
+(cheat)
+(form_goal 
+ “?!oleast:Pow(ordinal(A)) -> ordinal(A) +1.
+  (!s. (~(s = Empty(ordinal(A))) ==>
+     ?ord.App(i1(ordinal(A),1),ord) = App(oleast,s) &
+      IN(ord,s) &
+      !y. ordlt(y,ord) ==> ~IN(y,s))) &
+  App(oleast,Empty(ordinal(A))) = NONE(ordinal(A))  
+      ”)
+|> uex2ex_rule |> qSKOLEM "oleastf" [‘A’]
+
+val oleast_def = qdefine_fsym("oleast",[‘s:mem(Pow(ordinal(A)))’]) ‘App(oleastf(A),s)’
+
+val predsf_def = proved_th $
+e0
+cheat
+(form_goal “!A. ?!predf.
+ !alpha a:mem(ordinal(A)). IN(a,App(predf,alpha)) <=> ordlt(a,alpha) ”)
+|> spec_all |> uex2ex_rule |> qSKOLEM "predsf" [‘A’]
+
+val preds_def = 
+qdefine_fsym("preds",[‘alpha:mem(ordinal(A))’]) 
+‘App(predsf(A),alpha)’
+
+val sup_def = qdefine_fsym("sup",[‘s:mem(Pow(ordinal(A)))’])
+‘oleast(Compl(BIGUNION(IMAGE(predsf(A),s))))’
+|> gen_all
+
+val isomax_def = 
+qdefine_psym
+("isomax",[‘s:mem(Pow(ordinal(A)))’,‘ord:mem(ordinal(A))’])
+‘(IN(ord,s) & !y. ordlt(ord,y) ==> ~IN(y,s))’
+|> gen_all
+
+val omaxf_ex = proved_th $
+e0
+(cheat)
+(form_goal 
+ “?!omaxf:Pow(ordinal(A)) -> ordinal(A) +1.
+  (!s ord. isomax(s,ord) ==>
+           App(omaxf,s) = SOME(ord)) &
+  (!s. (!ord. ~isomax(s,ord)) ==> 
+    App(omaxf,s) = NONE(ordinal(A)))”)
+|> uex2ex_rule |> qSKOLEM "omaxf" [‘A’]
+
+val omax_def = qdefine_fsym("omax",[‘s:mem(Pow(ordinal(A)))’]) ‘App(omaxf(A),s)’
+
+
+val islimit_def = qdefine_psym("islimit",[‘alpha:mem(ordinal(A))’]) ‘omax(preds(alpha)) = NONE(ordinal(A))’ 
+
+val ordSUC_def = proved_th $
+e0
+cheat
+(form_goal “!A α:mem(ordinal(A)). ?!sα. ordlt(α,sα) &
+ !β. ordlt(α,β) ==> ordlt(sα,β) | sα = β”)
+|> spec_all |> uex2ex_rule |> qSKOLEM "ordSUC" [‘α’]
+
+
+
+
+(*
+val wobound_def = Define`
+  wobound x w = wellorder_ABS (rrestrict (wellorder_REP w) (iseg w x))
+`;*)
+
+
+
+
+val PSS_def = 
+qdefine_psym("PSS",[‘s1:mem(Pow(A))’,‘s2:mem(Pow(A))’])
+‘SS(s1,s2) & ~(s1 = s2)’ |> gen_all
+
+(*proper subsets*)
+val Pss_def =
+IN_def_P |> qspecl [‘Pow(A)’] 
+         |> fVar_sInst_th “P(a:mem(Pow(A)))”
+            “PSS(a,s0:mem(Pow(A)))”
+         |> uex2ex_rule 
+         |> qSKOLEM "Pss" [‘s0’]
+         |> gen_all
+
+
+val INmr_def = qdefine_psym("INmr",[‘a:mem(A)’,
+                                    ‘r:mem(Pow(A*A))’])
+‘?a1. IN(Pair(a,a1),r) | IN(Pair(a1,a),r)’ |> gen_all
+
+
+val INr_def = qdefine_psym("INr",[‘a:mem(A)’,‘R:A~>A’])
+‘?a1. Holds(R,a,a1) | Holds(R,a1,a)’
+
+val snocrel_def = 
+AX1 |> qspecl [‘A’,‘A’] 
+    |> fVar_sInst_th “P(a1:mem(A),a2:mem(A))”
+    “ Holds(R:A~>A,a1,a2) | (INr(a1,R) & a2 = a)”
+    |> uex2ex_rule |> qSKOLEM "snocrel" [‘R’,‘a’]
+    |> qspecl [‘a1:mem(A)’,‘a2:mem(A)’]
+    |> gen_all
+
+
+(*member to relation*)
+val m2r_def = AX1 |> qspecl [‘A’,‘A’]
+                  |> fVar_sInst_th “P(x:mem(A),y:mem(A))”
+                  “IN(Pair(x,y),od:mem(Pow(A * A)))”
+                  |> uex2ex_rule 
+                  |> qSKOLEM "m2r" [‘od’] 
+                  |> qspecl [‘a1:mem(A)’,‘a2:mem(A)’]
+                  |> gen_all
+
+
+val r2m_def = 
+    IN_def_P |> qspecl [‘A * A’]
+             |> fVar_sInst_th “P(a12:mem(A * A))”
+             “Holds(R:A~>A,Fst(a12),Snd(a12))” 
+             |> uex2ex_rule 
+             |> qSKOLEM "r2m" [‘R’] 
+             |> qspecl [‘Pair(a1:mem(A),a2:mem(A))’]
+             |> rewr_rule [Pair_def']
+             |> gen_all
+
+val snocm_def = qdefine_fsym("snocm",[‘r:mem(Pow(A * A))’,‘a:mem(A)’]) ‘r2m(snocrel(m2r(r),a))’ 
+ 
+
+(*do not really need the precondition, but want to make sure the condition is checked.*)
+val NOTINmr_snocm = prove_store("NOTINmr_snocm",
+e0
+(rpt strip_tac >> 
+rw[snocm_def,r2m_def,snocrel_def,m2r_def,INr_def,INmr_def])
+(form_goal
+ “!A r:mem(Pow(A*A)) a. ~INmr(a,r) ==>
+  !a1 a2. IN(Pair(a1,a2),snocm(r,a)) <=> 
+          IN(Pair(a1,a2),r) | (INmr(a1,r) & a2 = a)”));
+
+local
+val Wo_cl = 
+ “(od = Empty(A * A) ==> IN(od,wo)) &
+  (!od0 a.
+      IN(od0,wo) & ~INmr(a,od0) & od = snocm(od0,a) 
+      ==> IN(od,wo)) &
+  (!s. (!od0. IN(od0,s) ==> IN(od0,wo)) & 
+       SSchain(s) &
+       od = BIGUNION(s) ==>
+   IN(od,wo)) ”
+in
+val (Wo_incond,x1) = mk_incond Wo_cl;
+val Wof_ex = mk_fex Wo_incond x1;
+val Wof_def = mk_fdef "Wof" Wof_ex;
+val Wof_monotone = proved_th $
+e0
+(rpt strip_tac >>
+ rw[SS_def,Wof_def] >> rpt strip_tac (* 3 *)
+ >-- arw[] 
+ >-- (disj2_tac >> disj1_tac >>
+     qexistsl_tac [‘od0’,‘a'’] >> arw[] >>
+     fs[SS_def] >> first_x_assum irule >> arw[]) >>
+ disj2_tac >> disj2_tac >>
+ qexists_tac ‘s’ >> arw[] >> 
+ rpt strip_tac >> first_x_assum drule >>
+ fs[SS_def] >> first_x_assum irule >> arw[])
+(form_goal 
+“!s1 s2.SS(s1,s2) ==> 
+  SS(App(Wof(A), s1), App(Wof(A), s2))”)
+val Wo's_def = mk_prim Wof_def;
+val Wos_def = mk_LFP (rastt "Wo's(A)");
+val Wos_cond = mk_cond Wos_def Wo's_def;
+val Wos_SS = mk_SS Wos_def Wo's_def;
+val Wo_rules0 = mk_rules Wof_monotone Wos_SS Wos_cond;
+val Wo_cases0 = mk_cases Wof_monotone Wo_rules0 Wos_cond;
+val Wo_ind0 = mk_ind Wos_cond;
+val Wo_ind1 = mk_ind1 Wof_def Wo_ind0;
+val Wo_ind2 = mk_ind2 Wo_ind1;
+val Wo_cases1 = mk_case1 Wof_def Wo_cases0;
+val Wo_rules1 = mk_rules1 Wof_def Wo_rules0;
+val Wo_rules2 = mk_rules2 Wo_rules1;
+val Wo_rules3 = mk_rules3 Wo_rules2;
+end
+
+val oiso_def = 
+qdefine_psym("oiso",[‘f:A->B’,‘r1:mem(Pow(A*A))’,
+                              ‘r2:mem(Pow(B*B))’]) 
+‘!a1 a2. IN(Pair(a1,a2),r1) <=> IN()’
